Free CA

PartialCombinatoryAlgebras/FreeCombinatoryAlgebra.lean
@@ -1,9 +1,9 @@
 import PartialCombinatoryAlgebras.Basic
-import PartialCombinatoryAlgebras.PartialCombinatoryAlgebra
+import PartialCombinatoryAlgebras.CombinatoryAlgebra
 
 /-! # Free (total) combinatory algebra -/
 
-namespace FreeCombinatoryAlgebra
+namespace FreeCA
 
 /-- The underlying expressions fo the free combinatory algebra -/
 inductive Expr where
@@ -11,81 +11,65 @@ inductive Expr where
 | S : Expr
 | app : Expr → Expr → Expr
 
-instance Expr.hasDot : HasDot Expr where dot := app
+instance exprHasDot : HasDot Expr where dot := Expr.app
 
 /-- Provable equality on the free combinatory algebra -/
-inductive Expr.eq : Expr → Expr → Prop where
+inductive eq : Expr → Expr → Prop where
 | refl : ∀ {a}, eq a a
 | sym : ∀ {a b}, eq a b → eq b a
 | trans : ∀ {a b c}, eq a b → eq b c → eq a c
 | app : ∀ {a b c d}, eq a b → eq c d → eq (a ⬝ c) (b ⬝ d)
-| K : ∀ {a b}, eq (app (app K a) b) a
-| S : ∀ {a b c}, eq (app (app (app S a) b) c) (app (app a c) (app b c))
+| K : ∀ {a b}, eq (.app (.app .K a) b) a
+| S : ∀ {a b c}, eq (.app (.app (.app .S a) b) c) (.app (.app a c) (.app b c))
 
-infix:40 " ≈ " => Expr.eq
+@[inherit_doc]
+infix:40 " ≈ " => eq
 
 /-- The carrier of the free total combinatory algebra -/
-def carrier := Quot Expr.eq
+@[reducible]
+def carrier := Quot eq
 
 /-- Convert an expression to a (defined) partial element of the carrier. -/
 @[reducible]
-def mk (e : Expr) : Part carrier := Part.some (Quot.mk Expr.eq e)
+def mk := Quot.mk eq
+
+instance hasDot : HasDot carrier where
+  dot := Quot.lift₂ (fun (x y : Expr) => mk (x ⬝ y))
+    (by
+      intros a b c e'
+      apply Quot.sound
+      apply eq.app
+      · apply eq.refl
+      · assumption)
+    (by
+      intros a b c e'
+      apply Quot.sound
+      apply eq.app
+      · assumption
+      · apply eq.refl)
 
 @[simp]
-theorem df_mk (e : Expr) : (mk e) ⇓ := by trivial
+theorem eq_mk_app (a b : Expr) : mk a ⬝ mk b = mk (a ⬝ b) := by
+  simp [mk, hasDot]
 
-/-- Given a function `f : Expr → α` that preserves provable equality,
-    lift it to a function `∀ (u : Part carrier), u ⇓ → α. -/
-def lift {α : Sort} (f : Expr → α) (h : ∀ a b, a ≈ b → f a = f b) (u : Part carrier) (hu : u ⇓) : α :=
-  Quot.lift f h (u.get hu)
+end FreeCA
 
-def eq_lift {α : Sort} (f : Expr → α) (h : ∀ a b, a ≈ b → f a = f b) (e : Expr) :
-  lift f h (mk e) (df_mk e) = f e := by simp
+/-- Every combinatory algebra is a partial combinatory algebra -/
+instance FreeCA : CA FreeCA.carrier where
+  K := FreeCA.mk .K
+  S := FreeCA.mk .S
 
-/-- Given a function `f : Expr → Expr` that preserves provable equality,
-    convert it to a function on the partial elements of the carrier. -/
-def raise (f : Expr → Expr) (h : ∀ {a b}, a ≈ b → f a ≈ f b) (u : Part carrier) : Part carrier :=
-  Part.bind u (Quot.lift (fun (e : Expr) => mk (f e)) (fun a b h' => by simp ; apply Quot.sound ; apply h h'))
+  eq_K := by
+    apply Quot.ind ; intro a
+    apply Quot.ind ; intro b
+    rw [FreeCA.eq_mk_app, FreeCA.eq_mk_app]
+    apply Quot.sound
+    apply FreeCA.eq.K
 
-theorem eq_raise (f : Expr → Expr) (h : ∀ {a b}, a ≈ b → f a ≈ f b) (e : Expr) :
-  raise f h (mk e) = mk (f e) := by simp [raise]
-
-/-- Given a function `f : Expr → Expr → Expr` that preserves provable equality,
-    lift it to a function on the partial elements of the carrier. -/
-def raise₂ (f : Expr → Expr → Expr) (h : ∀ {a b c d}, a ≈ b → c ≈ d → f a c ≈ f b d) (u v : Part carrier) : Part carrier :=
-  Part.bind u (fun a =>
-    Part.bind v (fun b =>
-      Quot.lift₂
-        (fun x y => mk (f x y))
-        (fun a b₁ b₂ h' => by simp ; apply Quot.sound; apply h .refl h')
-        (fun a₁ a₂ b h' => by simp ; apply Quot.sound; apply h h' .refl)
-        a b
-    )
-  )
-
-theorem eq_raise₂ (f : Expr → Expr → Expr) (h : ∀ {a b c d}, a ≈ b → c ≈ d → f a c ≈ f b d) (a b : Expr) :
-  raise₂ f h (mk a) (mk b) = mk (f a b) := by simp [raise₂]
-
-instance CAisApplicativeStructure : PartialApplication carrier where
-  app := raise₂ Expr.app Expr.eq.app
-
-@[simp]
-theorem df_app (u v : Part carrier) : u ⇓ → v ⇓ → (u ⬝ v) ⇓ := by
-  intros hu hv
-  sorry
-
-instance CAisPCA : PCA carrier where
-  K := mk .K
-  S := mk .S
-
-  df_K₀ := by simp
-  df_K₁ hu := by simp [hu]
-  df_S₀ := by simp
-  df_S₁ hu := by simp [hu]
-  df_S₂ hu hv := by simp [hu, hv]
-
-  eq_K u v hu hv := by sorry
-
-  eq_S u v w _ _ _ := by sorry
-
-end FreeCombinatoryAlgebra
+  eq_S := by
+    apply Quot.ind ; intro a
+    apply Quot.ind ; intro b
+    apply Quot.ind ; intro c
+    rw [FreeCA.eq_mk_app, FreeCA.eq_mk_app, FreeCA.eq_mk_app]
+    apply Quot.sound
+    apply FreeCA.eq.S
